concrecte sorting algorithms beyond insertion sort
--HG--
extra : rebase_source : 36431fd18fc754577797c925fde167dd785eff3d

src/HOL/Library/Sorting_Algorithms.thy
@@ -6,11 +6,6 @@ theory Sorting_Algorithms
   imports Main Multiset Comparator
 begin
 
-text \<open>Prelude\<close>
-
-hide_const (open) sorted insort sort
-
-
 section \<open>Stably sorted lists\<close>
 
 abbreviation (input) stable_segment :: "'a comparator \<Rightarrow> 'a \<Rightarrow> 'a list \<Rightarrow> 'a list"
@@ -19,17 +14,26 @@ abbreviation (input) stable_segment :: "'a comparator \<Rightarrow> 'a \<Rightar
 fun sorted :: "'a comparator \<Rightarrow> 'a list \<Rightarrow> bool"
   where sorted_Nil: "sorted cmp [] \<longleftrightarrow> True"
   | sorted_single: "sorted cmp [x] \<longleftrightarrow> True"
-  | sorted_rec: "sorted cmp (y # x # xs) \<longleftrightarrow> compare cmp x y \<noteq> Less \<and> sorted cmp (x # xs)"
+  | sorted_rec: "sorted cmp (y # x # xs) \<longleftrightarrow> compare cmp y x \<noteq> Greater \<and> sorted cmp (x # xs)"
 
 lemma sorted_ConsI:
   "sorted cmp (x # xs)" if "sorted cmp xs"
-    and "\<And>y ys. xs = y # ys \<Longrightarrow> compare cmp y x \<noteq> Less"
+    and "\<And>y ys. xs = y # ys \<Longrightarrow> compare cmp x y \<noteq> Greater"
   using that by (cases xs) simp_all
+
+lemma sorted_Cons_imp_sorted:
+  "sorted cmp xs" if "sorted cmp (x # xs)"
+  using that by (cases xs) simp_all
+
+lemma sorted_Cons_imp_not_less:
+  "compare cmp y x \<noteq> Greater" if "sorted cmp (y # xs)"
+    and "x \<in> set xs"
+  using that by (induction xs arbitrary: y) (auto dest: compare.trans_not_greater)
 
 lemma sorted_induct [consumes 1, case_names Nil Cons, induct pred: sorted]:
   "P xs" if "sorted cmp xs" and "P []"
     and *: "\<And>x xs. sorted cmp xs \<Longrightarrow> P xs
-      \<Longrightarrow> (\<And>y. y \<in> set xs \<Longrightarrow> compare cmp y x \<noteq> Less) \<Longrightarrow> P (x # xs)"
+      \<Longrightarrow> (\<And>y. y \<in> set xs \<Longrightarrow> compare cmp x y \<noteq> Greater) \<Longrightarrow> P (x # xs)"
 using \<open>sorted cmp xs\<close> proof (induction xs)
   case Nil
   show ?case
@@ -40,7 +44,7 @@ next
     by (cases xs) simp_all
   moreover have "P xs" using \<open>sorted cmp xs\<close>
     by (rule Cons.IH)
-  moreover have "compare cmp y x \<noteq> Less" if "y \<in> set xs" for y
+  moreover have "compare cmp x y \<noteq> Greater" if "y \<in> set xs" for y
   using that \<open>sorted cmp (x # xs)\<close> proof (induction xs)
     case Nil
     then show ?case
@@ -54,10 +58,10 @@ next
         by simp
     next
       case (Cons w ws)
-      with Cons.prems have "compare cmp w z \<noteq> Less" "compare cmp z x \<noteq> Less"
+      with Cons.prems have "compare cmp z w \<noteq> Greater" "compare cmp x z \<noteq> Greater"
         by auto
-      then have "compare cmp w x \<noteq> Less"
-        by (auto dest: compare.trans_not_less)
+      then have "compare cmp x w \<noteq> Greater"
+        by (auto dest: compare.trans_not_greater)
       with Cons show ?thesis
         using Cons.prems Cons.IH by auto
     qed
@@ -69,7 +73,7 @@ qed
 lemma sorted_induct_remove1 [consumes 1, case_names Nil minimum]:
   "P xs" if "sorted cmp xs" and "P []"
     and *: "\<And>x xs. sorted cmp xs \<Longrightarrow> P (remove1 x xs)
-      \<Longrightarrow> x \<in> set xs \<Longrightarrow> hd (stable_segment cmp x xs) = x \<Longrightarrow> (\<And>y. y \<in> set xs \<Longrightarrow> compare cmp y x \<noteq> Less)
+      \<Longrightarrow> x \<in> set xs \<Longrightarrow> hd (stable_segment cmp x xs) = x \<Longrightarrow> (\<And>y. y \<in> set xs \<Longrightarrow> compare cmp x y \<noteq> Greater)
     \<Longrightarrow> P xs"
 using \<open>sorted cmp xs\<close> proof (induction xs)
   case Nil
@@ -80,7 +84,7 @@ next
   then have "sorted cmp (x # xs)"
     by (simp add: sorted_ConsI)
   moreover note Cons.IH
-  moreover have "\<And>y. compare cmp y x = Less \<Longrightarrow> y \<in> set xs \<Longrightarrow> False"
+  moreover have "\<And>y. compare cmp x y = Greater \<Longrightarrow> y \<in> set xs \<Longrightarrow> False"
     using Cons.hyps by simp
   ultimately show ?case
     by (auto intro!: * [of "x # xs" x]) blast
@@ -114,13 +118,27 @@ next
         assume "remove1 x ys = z # zs"
         with \<open>x \<noteq> y\<close> have "z \<in> set ys"
           using notin_set_remove1 [of z ys x] by auto
-        then show "compare cmp z y \<noteq> Less"
+        then show "compare cmp y z \<noteq> Greater"
           by (rule Cons.hyps(2))
       qed
       with False show ?thesis
         by simp
     qed
   qed
+qed
+
+lemma sorted_stable_segment:
+  "sorted cmp (stable_segment cmp x xs)"
+proof (induction xs)
+  case Nil
+  show ?case
+    by simp
+next
+  case (Cons y ys)
+  then show ?case
+    by (auto intro!: sorted_ConsI simp add: filter_eq_Cons_iff compare.sym)
+      (auto dest: compare.trans_equiv simp add: compare.sym compare.greater_iff_sym_less)
+
 qed
 
 primrec insort :: "'a comparator \<Rightarrow> 'a \<Rightarrow> 'a list \<Rightarrow> 'a list"
@@ -175,7 +193,7 @@ lemma remove1_insort_same_eq [simp]:
 
 lemma insort_eq_ConsI:
   "insort cmp x xs = x # xs"
-    if "sorted cmp xs" "\<And>y. y \<in> set xs \<Longrightarrow> compare cmp y x \<noteq> Less"
+    if "sorted cmp xs" "\<And>y. y \<in> set xs \<Longrightarrow> compare cmp x y \<noteq> Greater"
   using that by (induction xs) (simp_all add: compare.greater_iff_sym_less)
 
 lemma remove1_insort_not_same_eq [simp]:
@@ -188,14 +206,15 @@ using that proof (induction xs)
 next
   case (Cons z zs)
   show ?case
-  proof (cases "compare cmp z x = Less")
+  proof (cases "compare cmp x z = Greater")
     case True
     with Cons show ?thesis
-      by (simp add: compare.greater_iff_sym_less)
+      by simp
   next
     case False
-    have "compare cmp y x \<noteq> Less" if "y \<in> set zs" for y
-      using that False Cons.hyps by (auto dest: compare.trans_not_less)
+    then have "compare cmp x y \<noteq> Greater" if "y \<in> set zs" for y
+      using that Cons.hyps
+      by (auto dest: compare.trans_not_greater)
     with Cons show ?thesis
       by (simp add: insort_eq_ConsI)
   qed
@@ -211,7 +230,7 @@ using that proof (induction xs)
 next
   case (Cons y ys)
   then have "compare cmp x y \<noteq> Less"
-    by auto
+    by (auto simp add: compare.greater_iff_sym_less)
   then consider "compare cmp x y = Greater" | "compare cmp x y = Equiv"
     by (cases "compare cmp x y") auto
   then show ?case proof cases
@@ -225,6 +244,31 @@ next
     with Cons.hyps show ?thesis
       by (simp add: insort_eq_ConsI)
   qed
+qed
+
+lemma sorted_append_iff:
+  "sorted cmp (xs @ ys) \<longleftrightarrow> sorted cmp xs \<and> sorted cmp ys
+     \<and> (\<forall>x \<in> set xs. \<forall>y \<in> set ys. compare cmp x y \<noteq> Greater)" (is "?P \<longleftrightarrow> ?R \<and> ?S \<and> ?Q")
+proof
+  assume ?P
+  have ?R
+    using \<open>?P\<close> by (induction xs)
+      (auto simp add: sorted_Cons_imp_not_less,
+        auto simp add: sorted_Cons_imp_sorted intro: sorted_ConsI)
+  moreover have ?S
+    using \<open>?P\<close> by (induction xs) (auto dest: sorted_Cons_imp_sorted)
+  moreover have ?Q
+    using \<open>?P\<close> by (induction xs) (auto simp add: sorted_Cons_imp_not_less,
+      simp add: sorted_Cons_imp_sorted)
+  ultimately show "?R \<and> ?S \<and> ?Q"
+    by simp
+next
+  assume "?R \<and> ?S \<and> ?Q"
+  then have ?R ?S ?Q
+    by simp_all
+  then show ?P
+    by (induction xs)
+      (auto simp add: append_eq_Cons_conv intro!: sorted_ConsI)
 qed
 
 definition sort :: "'a comparator \<Rightarrow> 'a list \<Rightarrow> 'a list"
@@ -299,7 +343,7 @@ proof -
     case (minimum x xs)
     from \<open>mset ys = mset xs\<close> have ys: "set ys = set xs"
       by (rule mset_eq_setD)
-    then have "compare cmp y x \<noteq> Less" if "y \<in> set ys" for y
+    then have "compare cmp x y \<noteq> Greater" if "y \<in> set ys" for y
       using that minimum.hyps by simp
     from minimum.prems have stable: "stable_segment cmp x ys = stable_segment cmp x xs"
       by simp
@@ -317,5 +361,114 @@ proof -
     finally show ?case .
   qed
 qed
+
+lemma filter_insort:
+  "filter P (insort cmp x xs) = insort cmp x (filter P xs)"
+    if "sorted cmp xs" and "P x"
+  using that by (induction xs)
+    (auto simp add: compare.trans_not_greater insort_eq_ConsI)
+
+lemma filter_insort_triv:
+  "filter P (insort cmp x xs) = filter P xs"
+    if "\<not> P x"
+  using that by (induction xs) simp_all
+
+lemma filter_sort:
+  "filter P (sort cmp xs) = sort cmp (filter P xs)"
+  by (induction xs) (auto simp add: filter_insort filter_insort_triv)
+
+
+section \<open>Alternative sorting algorithms\<close>
+
+subsection \<open>Quicksort\<close>
+
+definition quicksort :: "'a comparator \<Rightarrow> 'a list \<Rightarrow> 'a list"
+  where quicksort_is_sort [simp]: "quicksort = sort"
+
+lemma sort_by_quicksort:
+  "sort = quicksort"
+  by simp
+
+lemma sort_by_quicksort_rec:
+  "sort cmp xs = sort cmp [x\<leftarrow>xs. compare cmp x (xs ! (length xs div 2)) = Less]
+    @ stable_segment cmp (xs ! (length xs div 2)) xs
+    @ sort cmp [x\<leftarrow>xs. compare cmp x (xs ! (length xs div 2)) = Greater]" (is "sort cmp ?lhs = ?rhs")
+proof (rule sort_eqI)
+  show "mset ?lhs = mset ?rhs"
+    by (rule multiset_eqI) (auto simp add: compare.sym intro: comp.exhaust)
+next
+  show "sorted cmp ?rhs"
+    by (auto simp add: sorted_append_iff sorted_stable_segment compare.equiv_subst_right dest: compare.trans_greater)
+next
+  let ?pivot = "xs ! (length xs div 2)"
+  fix l
+  assume "l \<in> set xs"
+  have "compare cmp x ?pivot = comp \<and> compare cmp l x = Equiv
+    \<longleftrightarrow> compare cmp l ?pivot = comp \<and> compare cmp l x = Equiv" for x comp
+  proof -
+    have "compare cmp x ?pivot = comp \<longleftrightarrow> compare cmp l ?pivot = comp"
+      if "compare cmp l x = Equiv"
+      using that by (simp add: compare.equiv_subst_left compare.sym)
+    then show ?thesis by blast
+  qed
+  then show "stable_segment cmp l ?lhs = stable_segment cmp l ?rhs"
+    by (simp add: stable_sort compare.sym [of _ ?pivot])
+      (cases "compare cmp l ?pivot", simp_all)
+qed
+
+context
+begin
+
+qualified definition partition :: "'a comparator \<Rightarrow> 'a \<Rightarrow> 'a list \<Rightarrow> 'a list \<times> 'a list \<times> 'a list"
+  where "partition cmp pivot xs =
+    ([x \<leftarrow> xs. compare cmp x pivot = Less], stable_segment cmp pivot xs, [x \<leftarrow> xs. compare cmp x pivot = Greater])"
+
+qualified lemma partition_code [code]:
+  "partition cmp pivot [] = ([], [], [])"
+  "partition cmp pivot (x # xs) =
+    (let (lts, eqs, gts) = partition cmp pivot xs
+     in case compare cmp x pivot of
+       Less \<Rightarrow> (x # lts, eqs, gts)
+     | Equiv \<Rightarrow> (lts, x # eqs, gts)
+     | Greater \<Rightarrow> (lts, eqs, x # gts))"
+  using comp.exhaust by (auto simp add: partition_def Let_def compare.sym [of _ pivot])
+
+lemma quicksort_code [code]:
+  "quicksort cmp xs =
+    (case xs of
+      [] \<Rightarrow> []
+    | [x] \<Rightarrow> xs
+    | [x, y] \<Rightarrow> (if compare cmp x y \<noteq> Greater then xs else [y, x])
+    | _ \<Rightarrow>
+        let (lts, eqs, gts) = partition cmp (xs ! (length xs div 2)) xs
+        in quicksort cmp lts @ eqs @ quicksort cmp gts)"
+proof (cases "length xs \<ge> 3")
+  case False
+  then have "length xs \<le> 2"
+    by simp
+  then have "length xs = 0 \<or> length xs = 1 \<or> length xs = 2"
+    using le_neq_trans less_2_cases by auto
+  then consider "xs = []" | x where "xs = [x]" | x y where "xs = [x, y]"
+    by (auto simp add: length_Suc_conv numeral_2_eq_2)
+  then show ?thesis
+    by cases simp_all
+next
+  case True
+  then obtain x y z zs where "xs = x # y # z # zs"
+    by (metis le_0_eq length_0_conv length_Cons list.exhaust not_less_eq_eq numeral_3_eq_3)
+  moreover have "quicksort cmp xs =
+    (let (lts, eqs, gts) = partition cmp (xs ! (length xs div 2)) xs
+    in quicksort cmp lts @ eqs @ quicksort cmp gts)"
+    using sort_by_quicksort_rec [of cmp xs] by (simp add: partition_def)
+  ultimately show ?thesis
+    by simp
+qed
+
+end
+
+text \<open>Evaluation example\<close>
+
+value "let cmp = key abs (reversed default)
+  in quicksort cmp [65, 1705, -2322, 734, 4, (-17::int)]"
 
 end
